src/int63/CnfInt63.v
@@ -84,7 +84,7 @@ Section Checker.
                 match (get_form (Lit.blit l1),get_form (Lit.blit l2)) with
                 | (Fatom a1,Fatom a2) =>
                   match (get_atom a1,get_atom a2) with
-                  | (Auop (UO_index x) j,Auop (UO_index y) k) => (j == i0-1)&&(k == j)
+                  | (Auop (UO_index x1) j,Auop (UO_index y1) k) => (j == i0-1)&&(k == j)&&(x == x1)&&(y==y1)
                   | _ => false
                   end
                 | _ => false
@@ -116,25 +116,21 @@ Definition check_BuildProjInt lits i :=
       match get_atom a with
       | Abop b h1 h2 => 
         match (b,get_atom h1,get_atom h2) with
-        | (BO_eq Tint,Acop (CO_int x),Acop (CO_int y)) => 
-          let fonction_map i l := if i == 0 then l else (if Lit.is_pos l then l else Lit.neg l) in
+        | (BO_eq t,Acop (CO_int x),Acop (CO_int y)) => 
+          let fonction_map i l := if Lit.is_pos l then l else Lit.neg l in
           let test_correct i0 l :=
-            if i0 == 0
-            then true
-            else (
-              match get_form (Lit.blit l) with
-              | Fiff l1 l2 =>
-                match (get_form (Lit.blit l1),get_form (Lit.blit l2)) with
-                | (Fatom a1,Fatom a2) =>
-                  match (get_atom a1,get_atom a2) with
-                  | (Auop (UO_index x) j,Auop (UO_index y) k) => (j == i0-1)&&(k == j)
-                  | _ => false
-                  end
+            match get_form (Lit.blit l) with
+            | Fiff l1 l2 =>
+              match (get_form (Lit.blit l1),get_form (Lit.blit l2)) with
+              | (Fatom a1,Fatom a2) =>
+                match (get_atom a1,get_atom a2) with
+                | (Auop (UO_index x1) j,Auop (UO_index y1) k) => (Lit.is_pos l1)&&(Lit.is_pos l2)&&(Typ.eqb t Typ.Tint)&&(j == i0)&&(k == j)&&(x == x1)&&(y==y1)
                 | _ => false
                 end
               | _ => false
               end
-                 )
+            | _ => false
+            end            
           in
           if test_correct i (lits.[i+1]) 
           then (fonction_map i (lits.[i+1]))::(Lit.nlit (Lit.blit (lits.[0])))::nil
@@ -149,4 +145,90 @@ Definition check_BuildProjInt lits i :=
   else C._true
   .
 
+
+
+
+Variable interp_atom : hatom -> bool.
+
+Local Notation rho := (Form.interp_state_var interp_atom t_form).
+
+Hypothesis Hch_f : check_form t_form.
+
+Check rho.
+
+Let Hwfrho : Valuation.wf rho.
+  Proof.
+    destruct (check_form_correct interp_atom _ Hch_f) as (_, H);exact H. 
+  Qed.
+
+
+Lemma lit_interp_true : Lit.interp rho Lit._true = true.
+  apply Lit.interp_true.
+  apply Hwfrho.
+Qed.
+
+
+Let rho_interp : forall x : int,
+    rho x = Form.interp interp_atom t_form (t_form.[ x]).
+  Proof.
+    destruct (check_form_correct interp_atom _ Hch_f) as ((H,H0), _).
+    intros x;apply wf_interp_form;trivial.
+  Qed.
+
+Lemma bool_impl : forall a b, (b = true -> a = true) -> a = true \/ b = false.
+Proof.
+intros.
+destruct a.
+left.
+trivial.
+right.
+destruct b.
+symmetry.
+apply H.
+trivial.
+trivial.
+Qed.
+
+Lemma lit_interp_impl : forall a b rho,(Lit.interp rho b = true -> Lit.interp rho a = true) -> (Lit.interp rho a =true \/Lit.interp rho (Lit.neg b) = true).
+Proof.
+  intros.
+  rewrite (Lit.interp_neg rho b).
+  rewrite negb_true_iff.
+  apply bool_impl.
+  apply H.
+Qed.
+
+
+Lemma valid_check_BuildProjInt : forall lits i, C.valid rho (check_BuildProjInt lits i).
+  Proof.
+   unfold check_BuildProjInt,C.valid;intros lits i.
+   case_eq ((length lits == digits + 1) && (i < digits)).
+
+   intros. case_eq (t_form.[Lit.blit (lits.[0])]).
+   intros. case_eq (t_atom.[i0]);intros; auto using C.interp_true.
+   case_eq b;intros; auto using C.interp_true.
+   case_eq (t_atom.[i1]);intros; auto using C.interp_true.
+   case_eq c;intros; auto using C.interp_true.
+   case_eq (t_atom.[i2]);intros; auto using C.interp_true.
+   case_eq c0;intros; auto using C.interp_true.
+   case_eq (t_form.[Lit.blit (lits.[i+1])]);intros;auto using C.interp_true.
+   case_eq (t_form.[Lit.blit i5]);intros;auto using C.interp_true.
+   case_eq (t_form.[Lit.blit i6]);intros;auto using C.interp_true.
+   case_eq (t_atom.[i7]);intros;auto using C.interp_true.
+   case_eq u;intros;auto using C.interp_true.
+   case_eq (t_atom.[i8]);intros;auto using C.interp_true.
+   case_eq u0;intros;auto using C.interp_true.
+   case_eq ((Lit.is_pos i5)&&(Lit.is_pos i6)&& Typ.eqb t Typ.Tint &&(i9 == i) && (i11 == i9) && (i3 == i10) && (i4 == i12));intros;case_eq (Lit.is_pos (lits.[i+1]));intros.
+   apply andb_true_iff in H14. destruct H14. apply andb_true_iff in H14. destruct H14. apply andb_true_iff in H14. destruct H14. apply andb_true_iff in H14. destruct H14. apply andb_true_iff in H14. destruct H14. apply andb_true_iff in H14. destruct H14.
+   simpl. rewrite orb_false_r. apply orb_true_iff. apply lit_interp_impl.
+   intro. 
+
+   unfold Lit.interp in H22. unfold Var.interp in H22. rewrite rho_interp in H22. rewrite Lit.is_pos_lit in H22. rewrite Lit.lit_blit in H22. rewrite H0 in H22.
+   unfold Lit.interp. unfold Var.interp. rewrite rho_interp. rewrite H15. rewrite H7.
+
+   unfold Form.interp. unfold Form.interp_aux. unfold Lit.interp. unfold Var.interp. rewrite H14. rewrite H21. rewrite rho_interp. rewrite H8. rewrite rho_interp. rewrite H9. unfold Form.interp. unfold Form.interp_aux. unfold Form.interp. unfold Form.interp_aux. unfold Form.interp in H22. unfold Form.interp_aux in H22.
+   SearchAbout interp_atom.
+  Qed.
  
+
+End Checker.
